ironfleet/src/Dafny/Distributed/Concur/Reduction.i.dfy
@@ -18,7 +18,6 @@ module ReductionModule
         && last(entries).end_group_level == entries[0].begin_group_level
         && GetEntryActor(last(entries).reduced_entry) == GetEntryActor(last(entries))
         && last(entries).reduced_entry.EntryAction?
-        && 0 < last(entries).pivot_index < |entries|
     }
 
     predicate EntriesReducibleToEntry(entries:seq<Entry>, entry:Entry)
@@ -31,11 +30,12 @@ module ReductionModule
     }
 
     predicate EntriesReducibleUsingPivot(entries:seq<Entry>)
-        requires EntryGroupValid(entries)
     {
-          var pivot := last(entries).pivot_index;
-          (forall i :: 0 <= i < pivot ==> EntryIsRightMover(entries[i]))
-       && (forall i :: pivot < i < |entries| ==> EntryIsLeftMover(entries[i]))
+          EntryGroupValid(entries)
+       && var pivot_index := last(entries).pivot_index;
+          0 < pivot_index < last(entries).group_len == |entries|
+       && (forall i :: 0 <= i < pivot_index ==> EntryIsRightMover(entries[i]))
+       && (forall i :: pivot_index < i < |entries| ==> EntryIsLeftMover(entries[i]))
     }
 
     function RestrictEntriesToLevel(entries:seq<Entry>, level:int) : Trace
@@ -65,10 +65,10 @@ module ReductionModule
            EntryGroupValid(entries)
         && min_level <= entries[0].begin_group_level < max_level
         && GetEntryLevel(last(entries).reduced_entry) == max_level
-        && ActorTraceValid(entries[1..|entries|-1], min_level, entries[0].begin_group_level)
-        && EntriesReducibleUsingPivot(entries)
-        && EntriesReducibleToEntry(RestrictEntriesToLevel(entries[1..|entries|-1], entries[0].begin_group_level),
-                                   last(entries).reduced_entry)
+        && var entries_restricted := RestrictEntriesToLevel(entries, entries[0].begin_group_level);
+           ActorTraceValid(middle(entries), min_level, entries[0].begin_group_level)
+        && EntriesReducibleUsingPivot(entries_restricted)
+        && EntriesReducibleToEntry(entries_restricted, last(entries).reduced_entry)
     }
 
     predicate ActorTraceValid(trace:Trace, min_level:int, max_level:int)
@@ -606,6 +606,7 @@ module ReductionModule
         db:seq<DistributedSystemState>,
         begin_entry_pos:int,
         end_entry_pos:int,
+        group:seq<Entry>,
         pivot_index:int,
         trace':Trace,
         db':seq<DistributedSystemState>,
@@ -615,12 +616,14 @@ module ReductionModule
         )
         requires IsValidDistributedSystemTraceAndBehavior(trace, db);
         requires 0 <= begin_entry_pos < end_entry_pos < |trace|;
-        requires EntryGroupValid(trace[begin_entry_pos .. end_entry_pos+1]);
-        requires EntriesReducibleUsingPivot(trace[begin_entry_pos .. end_entry_pos+1]);
-        requires pivot_index == trace[end_entry_pos].pivot_index;
+        requires group == trace[begin_entry_pos .. end_entry_pos+1];
+        requires EntryGroupValid(group);
+        requires group == RestrictEntriesToLevel(group, group[0].begin_group_level);
+        requires EntriesReducibleUsingPivot(group);
+        requires pivot_index == last(group).pivot_index;
         requires IsValidDistributedSystemTraceAndBehavior(trace', db');
         requires DistributedSystemBehaviorRefinesSpecBehavior(db', sb');
-        requires trace' == trace[..begin_entry_pos] + [trace[end_entry_pos].reduced_entry] + trace[end_entry_pos+1 ..];
+        requires trace' == trace[..begin_entry_pos] + [last(group).reduced_entry] + trace[end_entry_pos+1 ..];
         requires db' == db[..begin_entry_pos+1] + db[end_entry_pos+1 ..];
         requires sb ==   sb'[..begin_entry_pos]
                        + RepeatSpecState(sb'[begin_entry_pos], pivot_index + 1)
@@ -630,16 +633,23 @@ module ReductionModule
 
         ensures  SpecCorrespondence(db[i], sb[i]);
     {
+        lemma_ConcatenationOf4Sequences(sb'[..begin_entry_pos],
+                                        RepeatSpecState(sb'[begin_entry_pos], pivot_index + 1),
+                                        RepeatSpecState(sb'[begin_entry_pos+1], end_entry_pos - begin_entry_pos - pivot_index + 1),
+                                        sb'[begin_entry_pos+2..]);
+
         if i <= begin_entry_pos {
+            assert db'[i] == db[i];
+            assert sb'[i] == sb[i];
+            assert SpecCorrespondence(db'[i], sb'[i]);
             return;
         }
 
         assert i > 0;
         var ss := sb'[begin_entry_pos];
 
-        lemma_AddStuttersForReductionStepHelper1(trace, db, begin_entry_pos, end_entry_pos, pivot_index, trace', db', sb', sb, i-1);
+        lemma_AddStuttersForReductionStepHelper1(trace, db, begin_entry_pos, end_entry_pos, group, pivot_index, trace', db', sb', sb, i-1);
 
-        var group := trace[begin_entry_pos .. end_entry_pos+1];
         var k := i - 1;
         var j := k - begin_entry_pos;
         assert j >= 0;
@@ -648,21 +658,18 @@ module ReductionModule
         assert trace[k] == group[j];
         assert EntryIsRightMover(trace[k]);
         lemma_RightMoverForwardPreservation(trace[k], db[k], db[k+1], sb[k]);
+        assert SpecCorrespondence(db[k+1], sb[k]);
+        assert k+1 == i;
+        assert sb[i-1] == sb[i];
+        assert SpecCorrespondence(db[i], sb[i]);
     }
 
-    lemma seq_index_helper(s:seq, begin:int, end:int, absolute_index:int, relative_index:int)
-        requires 0 <= begin <= absolute_index <= end < |s|;
-        requires 0 <= relative_index < end - begin;
-        requires relative_index == absolute_index - begin;
-        ensures  s[begin..end][relative_index] == s[absolute_index];
-    {
-    }
-
-    lemma lemma_AddStuttersForReductionStepHelper2(
+    lemma {:timeLimitMultiplier 2} lemma_AddStuttersForReductionStepHelper2(
         trace:Trace,
         db:seq<DistributedSystemState>,
         begin_entry_pos:int,
         end_entry_pos:int,
+        group:seq<Entry>,
         pivot_index:int,
         trace':Trace,
         db':seq<DistributedSystemState>,
@@ -672,12 +679,14 @@ module ReductionModule
         )
         requires IsValidDistributedSystemTraceAndBehavior(trace, db);
         requires 0 <= begin_entry_pos < end_entry_pos < |trace|;
-        requires EntryGroupValid(trace[begin_entry_pos .. end_entry_pos+1]);
-        requires EntriesReducibleUsingPivot(trace[begin_entry_pos .. end_entry_pos+1]);
-        requires pivot_index == trace[end_entry_pos].pivot_index;
+        requires group == trace[begin_entry_pos .. end_entry_pos+1];
+        requires EntryGroupValid(group);
+        requires group == RestrictEntriesToLevel(group, group[0].begin_group_level);
+        requires EntriesReducibleUsingPivot(group);
+        requires pivot_index == last(group).pivot_index;
         requires IsValidDistributedSystemTraceAndBehavior(trace', db');
         requires DistributedSystemBehaviorRefinesSpecBehavior(db', sb');
-        requires trace' == trace[..begin_entry_pos] + [trace[end_entry_pos].reduced_entry] + trace[end_entry_pos+1 ..];
+        requires trace' == trace[..begin_entry_pos] + [last(group).reduced_entry] + trace[end_entry_pos+1 ..];
         requires db' == db[..begin_entry_pos+1] + db[end_entry_pos+1 ..];
         requires sb ==   sb'[..begin_entry_pos]
                        + RepeatSpecState(sb'[begin_entry_pos], pivot_index + 1)
@@ -690,7 +699,21 @@ module ReductionModule
     {
         if i >= end_entry_pos + 2 {
             assert |sb| == |sb'| + end_entry_pos - begin_entry_pos;
-            assert sb[i] == sb'[i-(end_entry_pos-begin_entry_pos)];
+            calc {
+                sb[i];
+                    { assert end_entry_pos + 2 == |sb'[..begin_entry_pos]|
+                        + |RepeatSpecState(sb'[begin_entry_pos], pivot_index + 1)|
+                        + |RepeatSpecState(sb'[begin_entry_pos+1], end_entry_pos - begin_entry_pos - pivot_index + 1)|; }
+                    { lemma_ConcatenationOf4Sequences(sb'[..begin_entry_pos],
+                                                      RepeatSpecState(sb'[begin_entry_pos], pivot_index + 1),
+                                                      RepeatSpecState(sb'[begin_entry_pos+1], end_entry_pos - begin_entry_pos - pivot_index + 1),
+                                                      sb'[begin_entry_pos+2..]); }
+                sb'[begin_entry_pos+2..][i - (end_entry_pos + 2)];
+                    { assert i - (end_entry_pos - begin_entry_pos) - (begin_entry_pos + 2) == i - (end_entry_pos + 2); }
+                sb'[begin_entry_pos+2..][i - (end_entry_pos - begin_entry_pos) - (begin_entry_pos + 2)];
+                    { lemma_ElementFromSequenceSuffix(sb', sb'[begin_entry_pos+2..], begin_entry_pos+2, i - (end_entry_pos - begin_entry_pos)); }
+                sb'[i-(end_entry_pos-begin_entry_pos)];
+            }
             return;
         }
         if i == end_entry_pos + 1 {
@@ -701,10 +724,9 @@ module ReductionModule
         var ss := sb'[begin_entry_pos];
         var ss' := sb'[begin_entry_pos+1];
 
-        lemma_AddStuttersForReductionStepHelper2(trace, db, begin_entry_pos, end_entry_pos, pivot_index, trace', db', sb', sb, i+1);
+        lemma_AddStuttersForReductionStepHelper2(trace, db, begin_entry_pos, end_entry_pos, group, pivot_index, trace', db', sb', sb, i+1);
 
         if begin_entry_pos + pivot_index < i < end_entry_pos + 1 {
-            var group := trace[begin_entry_pos .. end_entry_pos+1];
             lemma_ElementFromSequenceSlice(trace, group, begin_entry_pos, end_entry_pos+1, i);
             assert trace[i] == group[i - begin_entry_pos];
             assert EntryIsLeftMover(trace[i]);
@@ -739,6 +761,11 @@ module ReductionModule
         var ss' := sb'[begin_entry_pos+1];
         assert SpecNext(ss, ss') || ss == ss';
 
+        lemma_ConcatenationOf4Sequences(sb'[..begin_entry_pos],
+                                        RepeatSpecState(sb'[begin_entry_pos], pivot_index + 1),
+                                        RepeatSpecState(sb'[begin_entry_pos+1], end_entry_pos - begin_entry_pos - pivot_index + 1),
+                                        sb'[begin_entry_pos+2..]);
+
         if 0 <= i < begin_entry_pos - 1 {
             lemma_ElementFromSequencePrefix(sb', sb'[..begin_entry_pos], begin_entry_pos, i);
             lemma_ElementFromSequencePrefix(sb', sb'[..begin_entry_pos], begin_entry_pos, i+1);
@@ -754,6 +781,8 @@ module ReductionModule
             assert SpecNext(sb[i], sb[i+1]) || sb[i] == sb[i+1];
         }
         else if begin_entry_pos <= i < begin_entry_pos + pivot_index {
+            assert |sb'[..begin_entry_pos]| <= i < begin_entry_pos + pivot_index + 1 == |sb'[..begin_entry_pos]| + |RepeatSpecState(ss, pivot_index+1)|;
+            assert |sb'[..begin_entry_pos]| <= i + 1 < |sb'[..begin_entry_pos]| + |RepeatSpecState(ss, pivot_index+1)|;
             assert sb[i] == ss;
             assert sb[i+1] == ss;
         }
@@ -763,12 +792,30 @@ module ReductionModule
             assert SpecNext(sb[i], sb[i+1]) || sb[i] == sb[i+1];
         }
         else if begin_entry_pos + pivot_index < i <= end_entry_pos {
+            assert |sb'[..begin_entry_pos]| + |RepeatSpecState(ss, pivot_index+1)| <= i < |sb'[..begin_entry_pos]| + |RepeatSpecState(ss, pivot_index+1)| + |RepeatSpecState(ss', end_entry_pos - begin_entry_pos - pivot_index + 1)|;
+            assert |sb'[..begin_entry_pos]| + |RepeatSpecState(ss, pivot_index+1)| <= i + 1 < |sb'[..begin_entry_pos]| + |RepeatSpecState(ss, pivot_index+1)| + |RepeatSpecState(ss', end_entry_pos - begin_entry_pos - pivot_index + 1)|;
+            assert i > begin_entry_pos + pivot_index;
             assert sb[i] == ss';
             assert sb[i+1] == ss';
         }
+        else if i == end_entry_pos + 1 {
+            assert |sb'[..begin_entry_pos]| + |RepeatSpecState(ss, pivot_index+1)| <= i < |sb'[..begin_entry_pos]| + |RepeatSpecState(ss, pivot_index+1)| + |RepeatSpecState(ss', end_entry_pos - begin_entry_pos - pivot_index + 1)|;
+            assert sb[i] == ss' == sb'[begin_entry_pos+1];
+            assert |sb'[..begin_entry_pos]| + |RepeatSpecState(ss, pivot_index+1)| + |RepeatSpecState(ss', end_entry_pos - begin_entry_pos - pivot_index + 1)| <= i + 1;
+            assert sb[i+1] == sb'[begin_entry_pos+2];
+            assert SpecNext(sb'[begin_entry_pos+1], sb'[begin_entry_pos+1+1]) || sb'[begin_entry_pos+1] == sb'[begin_entry_pos+1+1];
+            assert SpecNext(sb[i], sb[i+1]) || sb[i] == sb[i+1];
+        }
         else {
-            assert end_entry_pos < i < |sb| - 1;
-            assert sb[i] == sb'[i - end_entry_pos + begin_entry_pos];
+            assert end_entry_pos + 2 == |sb'[..begin_entry_pos]| + |RepeatSpecState(ss, pivot_index+1)| + |RepeatSpecState(ss', end_entry_pos - begin_entry_pos - pivot_index + 1)| <= i < i + 1;
+            calc {
+                sb[i];
+                sb'[begin_entry_pos+2..][i - (end_entry_pos + 2)];
+                    { assert i - (end_entry_pos - begin_entry_pos) - (begin_entry_pos + 2) == i - (end_entry_pos + 2); }
+                sb'[begin_entry_pos+2..][i - (end_entry_pos - begin_entry_pos) - (begin_entry_pos + 2)];
+                    { lemma_ElementFromSequenceSuffix(sb', sb'[begin_entry_pos+2..], begin_entry_pos+2, i - (end_entry_pos - begin_entry_pos)); }
+                sb'[i-(end_entry_pos-begin_entry_pos)];
+            }
             assert sb[i+1] == sb'[i+1 - end_entry_pos + begin_entry_pos];
             var j := i - end_entry_pos + begin_entry_pos;
             assert SpecNext(sb'[j], sb'[j+1]) || sb'[j] == sb'[j+1];
@@ -776,11 +823,12 @@ module ReductionModule
         }
     }
 
-    lemma lemma_AddStuttersForReductionStep(
+    lemma {:timeLimitMultiplier 2} lemma_AddStuttersForReductionStep(
         trace:Trace,
         db:seq<DistributedSystemState>,
         begin_entry_pos:int,
         end_entry_pos:int,
+        group:seq<Entry>,
         trace':Trace,
         db':seq<DistributedSystemState>,
         sb':seq<SpecState>
@@ -789,32 +837,47 @@ module ReductionModule
         )
         requires IsValidDistributedSystemTraceAndBehavior(trace, db);
         requires 0 <= begin_entry_pos < end_entry_pos < |trace|;
-        requires EntryGroupValid(trace[begin_entry_pos .. end_entry_pos+1]);
-        requires EntriesReducibleUsingPivot(trace[begin_entry_pos .. end_entry_pos+1]);
+        requires group == trace[begin_entry_pos .. end_entry_pos+1];
+        requires EntryGroupValid(group);
+        requires group == RestrictEntriesToLevel(group, group[0].begin_group_level);
+        requires EntriesReducibleUsingPivot(group);
         requires IsValidDistributedSystemTraceAndBehavior(trace', db');
         requires DistributedSystemBehaviorRefinesSpecBehavior(db', sb');
-        requires trace' == trace[..begin_entry_pos] + [trace[end_entry_pos].reduced_entry] + trace[end_entry_pos+1 ..];
+        requires trace' == trace[..begin_entry_pos] + [last(group).reduced_entry] + trace[end_entry_pos+1 ..];
         requires db' == db[..begin_entry_pos+1] + db[end_entry_pos+1 ..];
 
         ensures  DistributedSystemBehaviorRefinesSpecBehavior(db, sb);
-        ensures  forall i :: begin_entry_pos <= i <= end_entry_pos && i != begin_entry_pos + trace[end_entry_pos].pivot_index ==> sb[i] == sb[i+1];
+        ensures  forall i :: begin_entry_pos <= i <= end_entry_pos && i != begin_entry_pos + last(group).pivot_index ==> sb[i] == sb[i+1];
     {
-        var pivot_index := trace[end_entry_pos].pivot_index;
+        var pivot_index := last(group).pivot_index;
         var entries := trace[begin_entry_pos+1 .. end_entry_pos];
         var ss := sb'[begin_entry_pos];
         var ss' := sb'[begin_entry_pos+1];
 
-        sb := sb'[..begin_entry_pos] + RepeatSpecState(ss, pivot_index + 1) + RepeatSpecState(ss', |entries| - pivot_index + 2) + sb'[begin_entry_pos+2..];
+        sb := sb'[..begin_entry_pos] + RepeatSpecState(ss, pivot_index + 1) + RepeatSpecState(ss', end_entry_pos - begin_entry_pos - pivot_index + 1) + sb'[begin_entry_pos+2..];
+
+        lemma_ConcatenationOf4Sequences(sb'[..begin_entry_pos],
+                                        RepeatSpecState(ss, pivot_index + 1),
+                                        RepeatSpecState(ss', end_entry_pos - begin_entry_pos - pivot_index + 1),
+                                        sb'[begin_entry_pos+2..]);
         assert |sb| == |sb'| + |entries| + 1 == |db|;
 
         forall i | begin_entry_pos <= i <= end_entry_pos && i != begin_entry_pos + pivot_index
             ensures sb[i] == sb[i+1];
         {
-            if i < begin_entry_pos + pivot_index {
+            if i == begin_entry_pos {
                 assert sb[i] == ss;
                 assert sb[i+1] == ss;
             }
+            else if i < begin_entry_pos + pivot_index {
+                assert |sb'[..begin_entry_pos]| <= i < begin_entry_pos + pivot_index + 1 == |sb'[..begin_entry_pos]| + |RepeatSpecState(ss, pivot_index+1)|;
+                assert sb[i] == RepeatSpecState(ss, pivot_index + 1)[i - begin_entry_pos];
+                assert sb[i] == ss;
+                assert |sb'[..begin_entry_pos]| <= i + 1 < begin_entry_pos + pivot_index + 1 == |sb'[..begin_entry_pos]| + |RepeatSpecState(ss, pivot_index+1)|;
+                assert sb[i+1] == ss;
+            }
             else {
+                assert |sb'[..begin_entry_pos]| + |RepeatSpecState(ss, pivot_index+1)| <= i < i + 1 < |sb'[..begin_entry_pos]| + |RepeatSpecState(ss, pivot_index+1)| + |RepeatSpecState(ss', end_entry_pos - begin_entry_pos - pivot_index + 1)|;
                 assert i > begin_entry_pos + pivot_index;
                 assert sb[i] == ss';
                 assert sb[i+1] == ss';
@@ -825,9 +888,9 @@ module ReductionModule
             ensures SpecCorrespondence(db[i], sb[i]);
         {
             if i <= begin_entry_pos + pivot_index {
-                lemma_AddStuttersForReductionStepHelper1(trace, db, begin_entry_pos, end_entry_pos, pivot_index, trace', db', sb', sb, i);
+                lemma_AddStuttersForReductionStepHelper1(trace, db, begin_entry_pos, end_entry_pos, group, pivot_index, trace', db', sb', sb, i);
             } else {
-                lemma_AddStuttersForReductionStepHelper2(trace, db, begin_entry_pos, end_entry_pos, pivot_index, trace', db', sb', sb, i);
+                lemma_AddStuttersForReductionStepHelper2(trace, db, begin_entry_pos, end_entry_pos, group, pivot_index, trace', db', sb', sb, i);
             } 
         }
 
@@ -838,13 +901,27 @@ module ReductionModule
         }
     }
 
-    lemma lemma_PerformOneReductionStep(
+    predicate DistributedSystemBehaviorRefinesSpecBehaviorWithConsecutiveNonPivotsAsStutters(
+        db:seq<DistributedSystemState>,
+        sb:seq<SpecState>,
+        begin_entry_pos:int,
+        end_entry_pos:int,
+        pivot_index:int
+        )
+    {
+           0 <= begin_entry_pos <= end_entry_pos < |sb|-1
+        && DistributedSystemBehaviorRefinesSpecBehavior(db, sb)
+        && forall i :: begin_entry_pos <= i <= end_entry_pos && i != begin_entry_pos + pivot_index ==> sb[i] == sb[i+1]
+    }
+
+    lemma {:timeLimitMultiplier 3} lemma_PerformOneReductionStep(
         trace:Trace,
         db:seq<DistributedSystemState>,
         actor:Actor,
         level:int,
         begin_entry_pos:int,
         end_entry_pos:int,
+        group:seq<Entry>,
         pivot_index:int
         ) returns (
         trace':Trace,
@@ -852,60 +929,59 @@ module ReductionModule
         )
         requires IsValidDistributedSystemTraceAndBehavior(trace, db);
         requires 0 <= begin_entry_pos < end_entry_pos < |trace|;
-        requires EntryGroupValid(trace[begin_entry_pos .. end_entry_pos+1]);
+        requires group == trace[begin_entry_pos .. end_entry_pos+1];
+        requires EntryGroupValid(group);
+        requires group == RestrictEntriesToLevel(group, group[0].begin_group_level);
         requires forall i :: begin_entry_pos < i < end_entry_pos ==> trace[i].EntryAction?;
         requires forall i :: begin_entry_pos <= i <= end_entry_pos ==> GetEntryActor(trace[i]) == actor;
         requires forall i :: begin_entry_pos <= i <= end_entry_pos ==> GetEntryLevel(trace[i]) == level;
-        requires EntriesReducibleUsingPivot(trace[begin_entry_pos .. end_entry_pos+1]);
-        requires EntriesReducibleToEntry(trace[begin_entry_pos+1 .. end_entry_pos], trace[end_entry_pos].reduced_entry);
-        requires pivot_index == trace[end_entry_pos].pivot_index;
+        requires EntriesReducibleUsingPivot(group);
+        requires EntriesReducibleToEntry(group, last(group).reduced_entry);
+        requires pivot_index == last(group).pivot_index;
         ensures  IsValidDistributedSystemTraceAndBehavior(trace', db');
         ensures  DistributedSystemBehaviorRefinesSpec(db')
-                 ==> exists sb :: DistributedSystemBehaviorRefinesSpecBehavior(db, sb) &&
-                            forall i :: begin_entry_pos <= i <= end_entry_pos && i != begin_entry_pos + pivot_index ==> sb[i] == sb[i+1];
-        ensures  trace' == trace[..begin_entry_pos] + [trace[end_entry_pos].reduced_entry] + trace[end_entry_pos+1 ..];
+                 ==> exists sb :: DistributedSystemBehaviorRefinesSpecBehaviorWithConsecutiveNonPivotsAsStutters(db, sb, begin_entry_pos, end_entry_pos, pivot_index);
+        ensures  trace' == trace[..begin_entry_pos] + [last(group).reduced_entry] + trace[end_entry_pos+1 ..];
     {
-        var entries := trace[begin_entry_pos .. end_entry_pos+1];
-        var reduced_entry := trace[end_entry_pos].reduced_entry;
+        var reduced_entry := last(group).reduced_entry;
         trace' := trace[..begin_entry_pos] + [reduced_entry] + trace[end_entry_pos+1 ..];
         db' := db[..begin_entry_pos+1] + db[end_entry_pos+1 ..];
 
-        var reducible_entries := trace[begin_entry_pos+1 .. end_entry_pos];
-        var tiny_db := db[begin_entry_pos+1 .. end_entry_pos+1];
-        assert |tiny_db| == |entries| - 1;
-        assert |tiny_db| == |reducible_entries| + 1;
-        forall i | 0 <= i < |tiny_db|-1
-            ensures DistributedSystemNextEntryAction(tiny_db[i], tiny_db[i+1], reducible_entries[i]);
+        var tiny_db := db[begin_entry_pos .. end_entry_pos+2];
+        assert |tiny_db| == |group| + 1;
+        forall i {:trigger DistributedSystemNextEntryAction(tiny_db[i], tiny_db[i+1], group[i])} | 0 <= i < |tiny_db|-1
+            ensures DistributedSystemNextEntryAction(tiny_db[i], tiny_db[i+1], group[i]);
         {
-            var j := i + begin_entry_pos + 1;
-            lemma_ElementFromSequenceSlice(trace, entries, begin_entry_pos, end_entry_pos+1, j);
-            assert trace[j] == entries[j - begin_entry_pos] == entries[i+1] == reducible_entries[i];
+            var j := i + begin_entry_pos;
+            lemma_ElementFromSequenceSlice(trace, group, begin_entry_pos, end_entry_pos+1, j);
+            assert trace[j] == group[j - begin_entry_pos] == group[i];
             assert DistributedSystemNextEntryAction(db[j], db[j+1], trace[j]);
-            lemma_ElementFromSequenceSlice(db, tiny_db, begin_entry_pos+1, end_entry_pos+1, j);
-            assert db[j] == tiny_db[j - (begin_entry_pos+1)] == tiny_db[i];
-            lemma_ElementFromSequenceSlice(db, tiny_db, begin_entry_pos+1, end_entry_pos+1, j+1);
-            assert db[j+1] == tiny_db[j+1 - (begin_entry_pos+1)] == tiny_db[i+1];
+            lemma_ElementFromSequenceSlice(db, tiny_db, begin_entry_pos, end_entry_pos+2, j);
+            assert db[j] == tiny_db[j - begin_entry_pos] == tiny_db[i];
+            lemma_ElementFromSequenceSlice(db, tiny_db, begin_entry_pos, end_entry_pos+2, j+1);
+            assert db[j+1] == tiny_db[j+1 - begin_entry_pos] == tiny_db[i+1];
         }
-        assert DistributedSystemNextEntryAction(tiny_db[0], tiny_db[|reducible_entries|], reduced_entry);
-
-        assert db[begin_entry_pos] == db[begin_entry_pos+1];
-        assert db[end_entry_pos] == db[end_entry_pos+1];
+        assert EntriesReducibleToEntry(group, reduced_entry);
+        assert DistributedSystemNextEntryAction(tiny_db[0], tiny_db[|group|], reduced_entry);
         assert DistributedSystemNextEntryAction(db'[begin_entry_pos], db'[begin_entry_pos+1], reduced_entry);
 
         forall i | 0 <= i < |trace'|
             ensures DistributedSystemNextEntryAction(db'[i], db'[i+1], trace'[i]);
         {
+            assert db'[i] == if i < begin_entry_pos+1 then db[i] else db[i + end_entry_pos - begin_entry_pos];
+            assert db'[i+1] == if i+1 < begin_entry_pos+1 then db[i+1] else db[i+1 + end_entry_pos - begin_entry_pos];
+            assert trace'[i] == if i < begin_entry_pos then trace[i] else if i == begin_entry_pos then reduced_entry else trace[i + end_entry_pos - begin_entry_pos];
         }
 
         assert IsValidDistributedSystemTraceAndBehavior(trace', db');
 
-        if sb' :| DistributedSystemBehaviorRefinesSpecBehavior(db', sb')
-        {
-            var sb := lemma_AddStuttersForReductionStep(trace, db, begin_entry_pos, end_entry_pos, trace', db', sb');
+        if DistributedSystemBehaviorRefinesSpec(db') {
+            var sb' :| DistributedSystemBehaviorRefinesSpecBehavior(db', sb');
+            var sb := lemma_AddStuttersForReductionStep(trace, db, begin_entry_pos, end_entry_pos, group, trace', db', sb');
             assert DistributedSystemBehaviorRefinesSpecBehavior(db, sb);
             assert forall i :: begin_entry_pos <= i <= end_entry_pos && i != begin_entry_pos + pivot_index ==> sb[i] == sb[i+1];
+            assert DistributedSystemBehaviorRefinesSpecBehaviorWithConsecutiveNonPivotsAsStutters(db, sb, begin_entry_pos, end_entry_pos, pivot_index);
         }
-
     }
 */
 }
